Fix interfaces
No proofs, only adjustments to the statements and identification of
missing results.

RSC_DC_MD_Instance.v
@@ -1,10 +1,13 @@
 Require Import RSC_DC_MD_Sigs.
 
+Require Import Common.CompCertExtensions.
+Require Import Common.TracesInform.
 Require Import Source.Language.
 Require Import Source.GlobalEnv.
 Require Import Source.CS.
 Require Import Source.Blame.
 Require Import Intermediate.Machine.
+Require Import Intermediate.CS.
 Require Import Intermediate.Recombination.
 Require Import S2I.Compiler.
 Require Import S2I.Definitions.
@@ -89,14 +92,20 @@ Module Intermediate_Instance <: Intermediate_Sig.
 
   Module CS.
     Definition sem :=
-      @Intermediate.CS.CS.sem.
+      @I.CS.sem_non_inform.
+
+    Definition sem_inform :=
+      @I.CS.sem_inform.
   End CS.
 
   Definition compose_mergeable_interfaces :=
     @Intermediate.compose_mergeable_interfaces.
 
   Definition recombination_prefix :=
-    @Intermediate.Recombination.recombination_prefix.
+    @Intermediate.Recombination.recombination_prefix_rel.
+
+  Definition does_prefix_inform_non_inform :=
+    @Intermediate.CS.CS.does_prefix_inform_non_inform.
 End Intermediate_Instance.
 
 Module S2I_Instance <: S2I_Sig (Source_Instance) (Intermediate_Instance).
